pulse/share/pulse/examples/parallel/Example.RingBufferTransfer.fst
@@ -1,0 +1,405 @@
+module Example.RingBufferTransfer
+open Pulse
+#lang-pulse
+open Pulse.Lib.Pervasives
+open FStar.Preorder
+module RB = Pulse.Lib.RingBuffer
+module MR = Pulse.Lib.MonotonicGhostRef
+module GR = Pulse.Lib.GhostReference
+module R = FStar.ReflexiveTransitiveClosure
+module L = Pulse.Lib.SpinLock
+let as_prop (p:Type) = p <==> True
+
+[@@erasable]
+noeq
+type stream (t:Type0) = {
+  messages: FStar.Seq.seq t;
+  read_position: i:nat { i <= Seq.length messages };
+}
+
+let empty_stream #t : stream t = { messages = Seq.empty; read_position = 0 }
+
+noeq
+type action (t:Type0) =
+| Send of t
+| Receive of t
+
+let send (#t:Type0) (m:t) (s0:stream t): stream t = { s0 with messages = Seq.snoc s0.messages m }
+
+let recv (#t:Type0) (s0:stream t) : GTot (option (t & stream t)) =
+  if s0.read_position < Seq.length s0.messages 
+  then Some (Seq.index s0.messages s0.read_position, { s0 with read_position = s0.read_position + 1 })
+  else None
+
+let receive (#t:Type0) (m:t) (s0:stream t) : stream t = snd (Some?.v (recv (send m s0)))
+
+let action_step (#t:Type0) (a:action t) (s0:stream t) (s1:stream t) : prop =
+  match a with
+  | Send m ->
+    s1 == send m s0
+  | Receive m ->
+    match recv s0 with
+    | None -> False
+    | Some (m', s1') -> m == m' /\ s1 == s1'
+
+let step (#t:Type0) (s0 s1:stream t) : prop = exists (a:action t). action_step #t a s0 s1
+let is_prefix #t : preorder (Seq.seq t) = fun s0 s1 ->
+  Seq.length s0 <= Seq.length s1 /\
+  Seq.slice s1 0 (Seq.length s0) `Seq.equal` s0
+let is_suffix_of #t (sfx s:Seq.seq t) : prop =
+  Seq.length sfx <= Seq.length s /\
+  Seq.slice s (Seq.length s - Seq.length sfx) (Seq.length s) `Seq.equal` sfx
+
+let suffix_of_reflexive #t (s:Seq.seq t) 
+: Lemma (s `is_suffix_of` s) = 
+  assert (Seq.append (Seq.empty) s `Seq.equal` s)
+
+let stream_evolves (#t:Type0) : preorder (stream t) = fun s0 s1 ->
+  R.closure (step #t) s0 s1 /\
+  is_prefix s0.messages s1.messages /\ //strengthened to make the proof of the main lemma easier
+  s0.read_position <= s1.read_position //strengthened to make the proof of the main lemma easier
+
+let stream_evolves_send #t (s0:stream t) (m:t)
+: Lemma (ensures stream_evolves #t s0 (send m s0))
+        [SMTPat (stream_evolves #t s0 (send m s0))]
+= assert (action_step #t (Send m) s0 (send m s0));
+  R.closure_step (step #t) s0 (send m s0)
+
+let incr_recv_position #t (s0:stream t{ s0.read_position < Seq.length s0.messages }) =
+  { s0 with read_position = s0.read_position + 1 }
+
+let stream_evolves_recv #t (s0:stream t)
+  : Lemma 
+    (requires s0.read_position < Seq.length s0.messages)
+    (ensures stream_evolves #t s0 (incr_recv_position s0))
+    [SMTPat (stream_evolves #t s0 (incr_recv_position s0))]
+  = assert (action_step #t (Receive (Seq.index s0.messages s0.read_position)) s0 (incr_recv_position s0));
+    R.closure_step (step #t) s0 (incr_recv_position s0)
+
+noeq
+type chan (t:Type0) = {
+  capacity: c:erased nat {c > 0}; //the capacity of the ring buffer, ghostly
+  buffer: RB.ringbuffer t; //the actual ring buffer
+  stream: MR.mref (stream_evolves #t);   //the entire stream, ghostly
+  read_position: GR.ref nat; //the current read position in the stream, ghostly
+  write_position: GR.ref nat; //the current write position in the stream, ghostly
+}
+
+let stream_exactly #t (c:chan t) (s:stream t) = MR.pts_to c.stream #1.0R s
+let stream_snapshot #t (c:chan t) (s:stream t) = MR.snapshot c.stream s
+
+[@@pulse_unfold]
+let channel_exactly #t ([@@@mkey] c:chan t) (s:stream t) =
+    stream_exactly c s ** //the ghost stream points exactly to s
+    GR.pts_to c.read_position #0.5R s.read_position ** //1/2 permission to the read position, agrees with s.read_position
+    GR.pts_to c.write_position #0.5R (Seq.length s.messages) ** //1/2 permission to the write position, agrees with s.read_position
+    (exists* suffix. 
+        RB.is_ringbuffer c.buffer suffix c.capacity //the buffer contains a suffix of the messages in s, with capacity c.capacity
+      ** pure (
+        suffix `is_suffix_of` s.messages /\
+        s.read_position == Seq.length s.messages - Seq.length suffix //the read position is exactly at the next message to be read
+      ) //and that suffix is indeed a suffix of s.messages
+    )
+
+
+noeq
+type channel (t:Type0) = {
+  ch:chan t;
+  l:L.lock;
+}
+
+let channel_perm #f (#t:Type0) (c:channel t) =
+  L.lock_alive c.l #f (exists* s. channel_exactly c.ch s)
+
+let reader_state (#t:Type0) (c:channel t) (s:stream t) =
+  exists* (s':stream t). 
+    stream_snapshot c.ch s' ** //knowledge of a stable snapshot
+    GR.pts_to c.ch.read_position #0.5R s.read_position ** //and 1/2 perm on the current read position
+    pure (s.messages `is_prefix` s'.messages /\ //and that snapshot's messages are an extension of the reader's current view
+          s.read_position == Seq.length s.messages /\
+          eq2 #nat s.read_position s'.read_position) //and everything in the reader's view has been read already
+
+let writer_state (#t:Type0) (c:channel t) (s:stream t) =
+  stream_snapshot c.ch s ** //knowledge of a stable snapshot
+  GR.pts_to c.ch.write_position #0.5R (Seq.length s.messages) //1/2 perm on the full stream
+
+ghost
+fn writer_has_full_knowledge_of_messages (#t:Type0) (c:channel t) (s s':stream t)
+  preserves writer_state c s
+  preserves GR.pts_to c.ch.write_position #0.5R (Seq.length s'.messages)
+  preserves stream_exactly c.ch s'
+  ensures pure (s.messages == s'.messages)
+{
+  unfold writer_state;
+  unfold stream_exactly;
+  unfold stream_snapshot;
+  MR.recall_snapshot _;
+  GR.pts_to_injective_eq c.ch.write_position;
+  assert pure (Seq.equal s.messages s'.messages);
+  fold stream_snapshot;
+  fold stream_exactly;
+  fold writer_state;
+}
+
+ghost
+fn reader_has_knowledge_of_prefix (#t:Type0) (c:channel t) (s s':stream t)
+  preserves reader_state c s
+  preserves exists* n. GR.pts_to c.ch.read_position #0.5R n ** pure (n == s'.read_position)
+  preserves stream_exactly c.ch s'
+  ensures pure (s.messages `is_prefix` s'.messages)
+  ensures pure (eq2 #nat s.read_position s'.read_position)
+{
+  unfold reader_state;
+  unfold stream_exactly;
+  unfold stream_snapshot;
+  MR.recall_snapshot _;
+  GR.pts_to_injective_eq c.ch.read_position;
+  fold stream_snapshot;
+  fold stream_exactly;
+  fold reader_state;
+}
+
+module SZ = FStar.SizeT
+
+fn create_channel (#t:Type0) (capacity:SZ.t{SZ.v capacity > 0}) (init:t)
+  returns c:channel t
+  ensures channel_perm #0.5R c
+  ensures channel_perm #0.5R c
+  ensures reader_state c empty_stream
+  ensures writer_state c empty_stream
+{
+  let buffer = RB.create capacity init;
+  let stream_ref = MR.alloc #_ #(stream_evolves #t) (empty_stream #t);
+  let read_pos = GR.alloc (0<:nat);
+  let write_pos = GR.alloc (0<:nat);
+  let ch = { 
+    capacity=SZ.v capacity; 
+    buffer;
+    stream = stream_ref;
+    read_position = read_pos;
+    write_position = write_pos 
+  };
+  rewrite each 
+    stream_ref as ch.stream, 
+    read_pos as ch.read_position,
+    write_pos as ch.write_position, 
+    buffer as ch.buffer;
+  MR.take_snapshot ch.stream _;
+  dup (MR.snapshot ch.stream (empty_stream #t)) ();
+  fold (stream_snapshot ch (empty_stream #t));
+  fold (stream_snapshot ch (empty_stream #t));
+  fold (stream_exactly ch (empty_stream #t));
+  GR.share ch.read_position;
+  GR.share ch.write_position;
+  suffix_of_reflexive (empty_stream #t).messages;
+  let lock = L.new_lock (exists* s. channel_exactly ch s);
+  let c = { ch; l = lock };
+  rewrite each ch as c.ch, lock as c.l;
+  L.share c.l;
+  fold (reader_state c (empty_stream #t));
+  fold (writer_state c (empty_stream #t));
+  fold (channel_perm #0.5R c);
+  fold (channel_perm #0.5R c);
+  c
+}
+
+fn destroy_channel_lock (#t:Type0) (c:channel t)
+  requires channel_perm #0.5R c ** channel_perm #0.5R c
+  ensures exists* s. channel_exactly c.ch s
+{
+  unfold channel_perm;
+  unfold channel_perm;
+  L.gather c.l;
+  L.acquire c.l;
+  L.free c.l;
+}
+
+fn destroy_channel #t (c:channel t)
+requires exists* s. channel_exactly c.ch s
+ensures emp
+{
+  RB.free c.ch.buffer;
+  drop_ (GR.pts_to c.ch.read_position #0.5R _);
+  drop_ (GR.pts_to c.ch.write_position #0.5R _);
+  drop_ (stream_exactly c.ch _);
+}
+
+fn rec write (#t:Type) (c:channel t) (m:t) (#s:stream t)
+  preserves channel_perm #0.5R c
+  requires writer_state c s
+  ensures exists* s'. writer_state c s' ** pure (s'.messages == (send m s).messages)
+{
+  unfold channel_perm;
+  L.acquire c.l;
+  let ok = RB.push_back c.ch.buffer m;
+  if not ok
+  { //no space left; recurse to retry
+    L.release c.l;
+    fold channel_perm;
+    write c m #s
+  }
+  else
+  {
+    writer_has_full_knowledge_of_messages c _ _;
+    unfold writer_state;
+    with s'. assert (stream_exactly c.ch s');
+    unfold stream_exactly;
+    GR.gather c.ch.write_position;
+    GR.write c.ch.write_position (Seq.length s.messages + 1);
+    GR.share c.ch.write_position;
+    MR.update c.ch.stream (send m s');
+    MR.take_snapshot c.ch.stream _;
+    drop_ (stream_snapshot c.ch s);
+    fold (stream_snapshot c.ch (send m s'));
+    fold (writer_state c (send m s'));
+    fold stream_exactly;
+    L.release c.l;
+    fold channel_perm;
+  }
+}
+
+fn rec read (#t:Type) (c:channel t) (#s:stream t)
+  preserves channel_perm #0.5R c
+  requires reader_state c s
+  returns m:t
+  ensures exists* s'. reader_state c s' ** pure (s' == receive m s)
+  
+{
+  unfold channel_perm;
+  L.acquire c.l;
+  if RB.is_empty c.ch.buffer
+  { //no messages to read; recurse to retry
+    L.release c.l;
+    fold channel_perm;
+    read c #s
+  }
+  else
+  {
+    let m = RB.peek_front c.ch.buffer;
+    RB.pop_front c.ch.buffer;
+    reader_has_knowledge_of_prefix c _ _;
+    unfold reader_state;
+    with s'. assert (stream_exactly c.ch s');
+    unfold stream_exactly;
+    GR.gather c.ch.read_position;
+    GR.write c.ch.read_position (s.read_position + 1);
+    GR.share c.ch.read_position;
+    MR.update c.ch.stream (incr_recv_position s');
+    MR.take_snapshot c.ch.stream _;
+    drop_ (stream_snapshot c.ch _);
+    fold (stream_snapshot c.ch (incr_recv_position s'));
+    fold (reader_state c (receive m s));
+    fold stream_exactly;
+    L.release c.l;
+    fold channel_perm;
+    m
+  }
+}
+
+
+ghost
+fn reader_writer_agree_on_prefix (#t:Type0) (c:channel t) (s0 s1 s2:stream t)
+  preserves reader_state c s0
+  preserves writer_state c s1
+  preserves channel_exactly c.ch s2
+  ensures pure (s0.messages `is_prefix` s1.messages /\ s1.messages == s2.messages)
+{
+  reader_has_knowledge_of_prefix c _ _;
+  writer_has_full_knowledge_of_messages c _ _;
+}
+
+ghost
+fn reader_writer_related (#t:Type0) (c:channel t) (s0 s1:stream t)
+  preserves reader_state c s0
+  preserves writer_state c s1
+  ensures pure (
+    //this is weaker than desired
+    //ideally we should be able to show without further assumptions that
+    //that only the LHS of the disjunct below is true
+    //For that, we would probably need to move to the Anchored preorders
+    //and prove that the write_state holds the anchor and so is
+    //always up to date... but that's for another revision
+    s0.messages `is_prefix` s1.messages \/
+    s1.messages `is_prefix` s0.messages
+  )
+{
+  unfold reader_state;
+  with s0'. assert (stream_snapshot c.ch s0');
+  unfold stream_snapshot;
+  unfold writer_state;
+  unfold stream_snapshot;
+  MR.snapshots_related c.ch.stream #s0' #s1;
+  fold (stream_snapshot c.ch s1);
+  fold writer_state;
+  fold (stream_snapshot c.ch s0');
+  fold reader_state;
+}
+
+///////////////////////////////////////////////////////////
+//A test program
+//Shows that you can create a channel,
+//spawn a reader and writer in parallel, and they will agree on the stream of messages
+///////////////////////////////////////////////////////////
+
+let is_id_seq_len (s:Seq.seq nat) (n:nat) : prop =
+  Seq.length s == n /\
+  (forall (i:nat { i < n }). Seq.index s i == i)
+
+fn writer (c:channel nat)
+  preserves channel_perm #0.5R c
+  requires writer_state c empty_stream
+  ensures exists* s'. writer_state c s' **
+    pure (is_id_seq_len s'.messages 50)
+{
+  let mut i : nat = 0;
+  while (!i < 50)
+  invariant live i
+  invariant (exists* s. writer_state c s ** pure (is_id_seq_len s.messages !i))
+  invariant pure (!i <= 50)
+  {
+    write c !i;
+    i := !i + 1;
+  };
+}
+
+fn reader (c:channel nat)
+  preserves channel_perm #0.5R c
+  requires reader_state c empty_stream
+  ensures exists* s'. reader_state c s' ** pure (Seq.length s'.messages == 50)
+{
+  let mut i : nat = 0;
+  while (!i < 50)
+  invariant live i
+  invariant (exists* s. reader_state c s ** pure (Seq.length s.messages == !i))
+  invariant pure (!i <= 50)
+  {
+    let _ = read c;
+    i := !i + 1;
+  };
+}
+
+//assume a primitive to spawn two threads in parallel and joining, similar to Pulse.Lib.Par
+fn par (#preL: slprop) #postL #preR #postR
+  (f:unit -> stt unit preL (fun _ -> postL))
+  (g:unit -> stt unit preR (fun _ -> postR))
+  requires preL
+  requires preR
+  ensures postL
+  ensures postR
+{ admit() }
+
+fn main ()
+{
+  let c = create_channel #nat 10sz 0; //create a channel with capacity 10
+  par (fun _ -> reader c) (fun _ -> writer c); //spawn a reader and writer in parallel; and wait for them to join
+  destroy_channel_lock c; //destroy the channel, ensuring all resources are cleaned up
+  reader_writer_agree_on_prefix c _ _ _; //at this point we can prove using this ghost function
+  assert (exists* s0 s1.  //that the reader and writer agree on the entire stream of messages
+    reader_state c s0 **
+    writer_state c s1 ** 
+    pure (Seq.equal s0.messages s1.messages)); //and that stream contains exactly the messages we expect
+  //free up rest
+  destroy_channel c;
+  drop_ (reader_state c _);
+  drop_ (writer_state c _);
+}
